src/verification/semantics/add.lean
@@ -1,0 +1,200 @@
+import verification.semantics.skip_stream
+
+/-!
+# Addition of indexed streams
+
+In this file, we define the sum of indexed streams `Stream.add`.
+
+## Main results
+  - `add_spec`: States that `(a.add b).eval q = (a.eval q) + (b.eval q)` i.e. 
+      add does what it says it does, assuming `a` and `b` are lawful (note that we
+      do not need to assume strict lawfulness).
+  - `is_lawful (a.add b)`: The sum stream is lawful assuming `a` and `b` are.
+  - `is_strict_lawful (a.add b)`: The sum stream is strictly lawful assuming `a` and `b` are.
+-/
+
+noncomputable theory
+open_locale streams
+variables {ι : Type} [linear_order ι] {α : Type*}
+
+@[simps] def Stream.add [has_zero α] [has_add α] (a b : Stream ι α) : Stream ι α :=
+{ σ := a.σ × b.σ,
+  valid := λ s, a.valid s.1 ∨ b.valid s.2,
+  ready := λ s, (a.to_order' s.1 ≤ b.to_order' s.2 ∧ a.ready s.1) ∨ (b.to_order' s.2 ≤ a.to_order' s.1 ∧ b.ready s.2),
+  skip := λ p hp i, (a.skip' p.1 i, b.skip' p.2 i),
+  index := λ s h, option.get (show (min (a.index' s.1) (b.index' s.2)).is_some, by simpa),
+  value := λ s h, (if a.to_order' s.1 ≤ b.to_order' s.2 then a.value' s.1 else 0) +
+                  (if b.to_order' s.2 ≤ a.to_order' s.1 then b.value' s.2 else 0) } 
+
+section index_lemmas
+variables [has_zero α] [has_add α]
+
+@[simp] lemma add_index_eq_min {a b : Stream ι α} (q : (a.add b).σ) :
+  (a.add b).index' q = min (a.index' q.1) (b.index' q.2) :=
+by { by_cases H : (a.add b).valid q, { simp [H], }, { simp [H, not_or_distrib.mp H], } }
+
+lemma valid_of_to_order_lt {a b : Stream ι α} {qa : a.σ} {qb : b.σ} (h : a.to_order' qa < b.to_order' qb) :
+  a.valid qa :=
+by { contrapose! h, by_cases hb : b.valid qb, { rw prod.lex.le_iff', left, simpa [h], }, { simp [Stream.to_order', h, hb], } }
+
+@[simp] lemma add_skip_fst {a b : Stream ι α} (q i) : ((a.add b).skip' q i).fst = a.skip' q.1 i :=
+by { simp only [Stream.skip'], split_ifs with h₁ h₂ h₂, { simp [h₂], }, { simp [h₂], }, { cases h₁ (or.inl h₂), }, { refl, }, }
+
+@[simp] lemma add_skip_snd {a b : Stream ι α} (q i) : ((a.add b).skip' q i).snd = b.skip' q.2 i :=
+by { simp only [Stream.skip'], split_ifs with h₁ h₂ h₂, { simp [h₂], }, { simp [h₂], }, { cases h₁ (or.inr h₂), }, { refl, }, }
+
+lemma of_to_order_eq {a b : Stream ι α} (q : (a.add b).σ) (h : a.to_order' q.1 = b.to_order' q.2) :
+  (¬((a.add b).valid q) ∧ ¬(a.valid q.1) ∧ ¬(b.valid q.2)) ∨
+  ((a.add b).valid q ∧ a.valid q.1 ∧ b.valid q.2 ∧ (a.ready q.1 ↔ b.ready q.2) ∧ a.index' q.1 = b.index' q.2) :=
+begin
+  have : a.index' q.1 = b.index' q.2 := by simpa using congr_arg prod.fst h,
+  by_cases H : (a.add b).valid q,
+  { right, 
+    obtain ⟨hv₁, hv₂⟩ : a.valid q.1 ∧ b.valid q.2, { simp only [← Stream.index'_lt_top_iff] at H ⊢, simpa [this, -Stream.index'_lt_top_iff] using H, },
+    refine ⟨H, hv₁, hv₂, _, this⟩,
+    simpa [hv₁, hv₂] using congr_arg prod.snd h, },
+  { left, refine ⟨H, not_or_distrib.mp H⟩, },
+end
+
+lemma add_to_order_eq_min {a b : Stream ι α} (q : (a.add b).σ) :
+  (a.add b).to_order' q = min (a.to_order' q.1) (b.to_order' q.2) :=
+begin
+  rcases lt_trichotomy (a.to_order' q.1) (b.to_order' q.2) with (h|h|h),
+  { rw min_eq_left h.le, ext : 1,
+    { simpa using prod.lex.fst_le_of_le h.le, },
+    { simp [valid_of_to_order_lt h, h.le, h.not_le], }, },
+  { rcases of_to_order_eq _ h with (⟨H, hv₁, hv₂⟩|⟨H, hv₁, hv₂, hr, hi⟩),
+    { simp [Stream.to_order', H, hv₁, hv₂], },
+    ext : 1, { simp [h, hi], }, simp [Stream.to_order'_val_snd H, h, Stream.to_order'_val_snd hv₂, hr], },
+  { rw min_eq_right h.le, ext : 1,
+    { simpa using prod.lex.fst_le_of_le h.le, },
+    { simp [valid_of_to_order_lt h, h.le, h.not_le], }, },
+end
+
+lemma add_to_order_left {a b : Stream ι α} {q : (a.add b).σ} (hq hq') (ha : a.to_order' q.1 ≤ b.to_order' q.2) :
+  (a.add b).to_order q hq = a.to_order q.1 hq' :=
+coe_lex_injective (by simpa [add_to_order_eq_min])
+
+lemma add_to_order_right {a b : Stream ι α} {q : (a.add b).σ} (hq hq') (ha : b.to_order' q.2 ≤ a.to_order' q.1) :
+  (a.add b).to_order q hq = b.to_order q.2 hq' :=
+coe_lex_injective (by simpa [add_to_order_eq_min])
+
+instance Stream.add.is_bounded (a b : Stream ι α) [is_bounded a] [is_bounded b] : is_bounded (a.add b) :=
+is_bounded.mk' ⟨prod.rprod_eq a.wf_rel b.wf_rel, prod.rprod_eq_wf a.wf b.wf, λ q i, begin
+  rcases a.wf_valid' q.1 i with (h|⟨ha₁, ha₂⟩),
+  { left, left, simp only [add_skip_fst, add_skip_snd], exact ⟨h, (b.wf_valid' q.2 i).imp_right and.right⟩, },
+  rcases b.wf_valid' q.2 i with (h|⟨hb₁, hb₂⟩),
+  { left, right, simp only [add_skip_fst, add_skip_snd], exact ⟨h, (a.wf_valid' q.1 i).imp_right and.right⟩, },
+  right, split,
+  { rw [add_to_order_eq_min, lt_min_iff], split; assumption, }, { ext; simpa, }
+end⟩
+
+lemma add_mono {a b : Stream ι α}  (ha : a.is_monotonic) (hb : b.is_monotonic) : (a.add b).is_monotonic :=
+by { intros q hv i, simp only [add_index_eq_min], exact min_le_min (ha.skip' _ _) (hb.skip' _ _), }
+
+lemma add_strict_mono {a b : Stream ι α} (ha : a.is_strict_mono) (hb : b.is_strict_mono) : (a.add b).is_strict_mono :=
+⟨add_mono ha.1 hb.1, λ q hq i hi hr, ne_of_lt begin
+  replace hi : min (a.to_order' q.1) (b.to_order' q.2) ≤ coe_lex i, { rwa [← add_to_order_eq_min, ← Stream.coe_lex_to_order hq, coe_lex_le_iff], },
+  rcases (lt_trichotomy (a.to_order' q.1) (b.to_order' q.2)) with (h|h|h),
+  { replace hr : a.ready q.1 := by simpa [h.le, h.not_le] using hr,
+    have hqa : a.valid q.1 := valid_of_to_order_lt h,
+    replace hi : a.to_order q.1 hqa ≤ i, { rw [min_eq_left h.le] at hi, rwa [← coe_lex_le_iff, Stream.coe_lex_to_order], }, 
+    have : a.index' q.1 < b.index' q.2, { refine prod.lex.fst_lt_of_lt_of_le h _, simp [hqa, hr], },
+    simp only [add_index_eq_min, min_eq_left this.le, Stream.add_skip, add_index_eq_min, lt_min_iff, Stream.skip'_val hqa],
+    split, { exact ha.lt _ _ _ hi hr, }, { refine this.trans_le _, apply hb.1.skip', }, },
+  { obtain ⟨hv₀, hv₁, hv₂, hr_iff, hind⟩ := (of_to_order_eq _ h).resolve_left (λ h', h'.1 hq),
+    simp only [add_index_eq_min, hind, min_self, Stream.add_skip, lt_min_iff],
+    obtain ⟨hr₁, hr₂⟩ : a.ready q.1 ∧ b.ready q.2, { split; simpa [h, hr_iff] using hr, }, 
+    split,
+    { rw [← hind, Stream.skip'_val hv₁], rw [← h, min_self, ← Stream.coe_lex_to_order hv₁, coe_lex_le_iff] at hi, exact ha.lt _ _ _ hi hr₁, },
+    { rw [Stream.skip'_val hv₂], rw [h, min_self, ← Stream.coe_lex_to_order hv₂, coe_lex_le_iff] at hi, exact hb.lt _ _ _ hi hr₂, }, },
+  { replace hr : b.ready q.2 := by simpa [h.le, h.not_le] using hr,
+    have hqb : b.valid q.2 := valid_of_to_order_lt h,
+    replace hi : b.to_order q.2 hqb ≤ i, { rw [min_eq_right h.le] at hi, rwa [← coe_lex_le_iff, Stream.coe_lex_to_order], }, 
+    have : b.index' q.2 < a.index' q.1, { refine prod.lex.fst_lt_of_lt_of_le h _, simp [hqb, hr], },
+    simp only [add_index_eq_min, min_eq_right this.le, Stream.add_skip, add_index_eq_min, lt_min_iff, Stream.skip'_val hqb],
+    split, swap, { exact hb.lt _ _ _ hi hr, }, { refine this.trans_le _, apply ha.1.skip', }, },
+end⟩
+
+lemma Stream.add_map {β : Type*} [has_zero β] [has_add β] (f : α → β) (f_add : ∀ x y, f (x + y) = f x + f y)
+  (f_zero : f 0 = 0) (q r : Stream ι α) : (q.add r).map f = ((q.map f).add (r.map f)) :=
+by { ext; solve_refl, simp only [f_add, apply_ite f, f_zero, Stream.map_value' f f_zero], }
+
+end index_lemmas
+
+section value_lemmas
+variables [add_comm_monoid α]
+
+lemma Stream.add.eval₀_eq_left {a b : Stream ι α} {q : (a.add b).σ} (hq : (a.add b).valid q) (H : a.to_order' q.1 < b.to_order' q.2) :
+  (a.add b).eval₀ q hq = a.eval₀ q.1 (valid_of_to_order_lt H) :=
+begin
+  have := add_to_order_left hq (valid_of_to_order_lt H) H.le,
+  have hr : (a.add b).ready q ↔ a.ready q.1, { simpa using congr_arg prod.snd this, },
+  simp only [Stream.eval₀, ← Stream.value'_val, dite_eq_ite], rw [hr],
+  split_ifs with hr', swap, { refl, },
+  congr' 1, { simpa using congr_arg prod.fst this, },
+  simp [@Stream.value'_val _ _ _ (a.add b) _ (or.inl ⟨H.le, hr'⟩), H.le, H.not_le],
+end
+
+lemma Stream.add.eval₀_eq_right {a b : Stream ι α} {q : (a.add b).σ} (hq : (a.add b).valid q) (H : b.to_order' q.2 < a.to_order' q.1) :
+  (a.add b).eval₀ q hq = b.eval₀ q.2 (valid_of_to_order_lt H) :=
+begin
+  have := add_to_order_right hq (valid_of_to_order_lt H) H.le,
+  have hr : (a.add b).ready q ↔ b.ready q.2, { simpa using congr_arg prod.snd this, },
+  simp only [Stream.eval₀, ← Stream.value'_val, dite_eq_ite], rw [hr],
+  split_ifs with hr', swap, { refl, },
+  congr' 1, { simpa using congr_arg prod.fst this, },
+  simp [@Stream.value'_val _ _ _ (a.add b) _ (or.inr ⟨H.le, hr'⟩), H.le, H.not_le],
+end
+
+lemma Stream.add.eval₀_eq_both {a b : Stream ι α} {q : (a.add b).σ} (hq : (a.add b).valid q) (H : a.to_order' q.1 = b.to_order' q.2) (hv₁ hv₂) (hr : a.ready q.1 ↔ b.ready q.2) 
+  (hi : a.index q.1 hv₁ = b.index q.2 hv₂) : (a.add b).eval₀ q hq = a.eval₀ q.1 hv₁ + b.eval₀ q.2 hv₂ :=
+begin
+  have : (a.add b).ready q ↔ b.ready q.2, { simp [H, hr], },
+  simp only [Stream.eval₀, ← Stream.value'_val, dite_eq_ite], rw [this, hr],
+  split_ifs with hr', swap, { simp, },
+  rw [hi, ← finsupp.single_add, Stream.add_index, @Stream.value'_val _ _ _ (a.add b)],
+  { simp [Stream.index'_val hv₁, Stream.index'_val hv₂, hi, -finsupp.single_add, H], },
+  right, refine ⟨_, hr'⟩, rw [H],
+end
+
+lemma add_spec (a b : Stream ι α) [is_lawful a] [is_lawful b] (q : (a.add b).σ) :
+  (a.add b).eval q = (a.eval q.1) + (b.eval q.2) :=
+begin
+  refine @well_founded.induction _ (a.add b).wf_rel (a.add b).wf _ q _,
+  clear q, intros q ih,
+  rcases lt_trichotomy (a.to_order' q.1) (b.to_order' q.2) with (h|h|h),
+  { have hv : a.valid q.1 := valid_of_to_order_lt h,
+    have hq : (a.add b).valid q := or.inl hv,
+    rw [(a.add b).eval_valid q hq, ih _ ((a.add b).next_wf _ hq), Stream.next_val hq, Stream.add_skip, @Stream.skip'_lt_to_order _ _ _ _ b,
+      add_to_order_left hq hv h.le, Stream.skip'_val hv, a.eval_valid _ hv, add_assoc, Stream.add.eval₀_eq_left hq h, Stream.next_val hv],
+    simpa [add_to_order_eq_min], },
+  { rcases of_to_order_eq _ h with (⟨H, hv₁, hv₂⟩|⟨hq, hv₁, hv₂, hr, hi⟩),
+    { simp [H, hv₁, hv₂], },
+    obtain ⟨t₀, t₁⟩ : (a.add b).to_order q hq = a.to_order q.1 hv₁ ∧ (a.add b).to_order q hq = b.to_order q.2 hv₂,
+    { split; apply_fun coe_lex using coe_lex_injective; simp [add_to_order_eq_min, h], },
+    simp only [Stream.index'_val, hv₁, hv₂, with_top.coe_eq_coe] at hi,
+    rw [(a.add b).eval_valid q hq, ih _ ((a.add b).next_wf _ hq), Stream.next_val hq, Stream.add_skip, Stream.add.eval₀_eq_both hq h hv₁ hv₂ hr hi,
+      (show ∀ (w x y z : ι →₀ α), (w + x) + (y + z) = (w + y) + (x + z), by intros; abel)], dsimp only,
+    congr' 1,
+    { rw [a.eval_valid _ hv₁, Stream.next_val hv₁, t₀, Stream.skip'_val hv₁], },
+    { rw [b.eval_valid _ hv₂, Stream.next_val hv₂, t₁, Stream.skip'_val hv₂], }, },
+  { have hv : b.valid q.2 := valid_of_to_order_lt h,
+    have hq : (a.add b).valid q := or.inr hv,
+    rw [(a.add b).eval_valid q hq, ih _ ((a.add b).next_wf _ hq), Stream.next_val hq, Stream.add_skip, @Stream.skip'_lt_to_order _ _ _ _ a,
+      add_to_order_right hq hv h.le, Stream.skip'_val hv, b.eval_valid _ hv, add_left_comm, Stream.add.eval₀_eq_right hq h, Stream.next_val hv],
+    simpa [add_to_order_eq_min], },
+end
+
+instance (a b : Stream ι α) [is_lawful a] [is_lawful b] : is_lawful (a.add b) :=
+⟨add_mono a.mono b.mono, λ q hq i j hj, begin
+  simp only [add_spec], dsimp,
+  congr' 1; rwa Stream.skip'_spec,
+end⟩
+
+instance (a b : Stream ι α) [is_strict_lawful a] [is_strict_lawful b] : is_strict_lawful (a.add b) :=
+{ strict_mono := add_strict_mono a.strict_mono b.strict_mono }
+
+end value_lemmas
+
+
