src/verification/semantics/contract.lean
@@ -1,0 +1,77 @@
+import verification.semantics.skip_stream
+
+/-!
+# Contraction of indexed streams
+
+In this file, we define the contraction of indexed streams `Stream.contract`.
+This replaces the indexing axis with `() : Unit`, implicitly summing over the
+values of the stream.
+
+## Main results
+  - `contract_eval`: Correctness for `contract`; evaluating `contract s` results in
+    the sum of the values of `s`
+  - `is_lawful (Stream.contract s)`: `s.contract` is lawful assuming `s` is
+
+-/
+
+variables {ι : Type} {α : Type*}
+
+@[simps] def Stream.contract (s : Stream ι α) : Stream unit α :=
+{ σ := s.σ,
+  valid := s.valid,
+  ready := s.ready,
+  skip := λ q hq i, s.skip q hq (s.index q hq, i.2),
+  index := default,
+  value := s.value }
+
+variables [linear_order ι]
+
+section index_lemmas
+
+instance (s : Stream ι α) [is_bounded s] : is_bounded (Stream.contract s) :=
+⟨⟨s.wf_rel, s.wf, λ q hq, begin
+  rintro ⟨⟨⟩, b⟩,
+  simp only [Stream.contract_skip],
+  refine (s.wf_valid q hq (s.index q hq, b)).imp_right (and.imp_left _),
+  simp [Stream.to_order], exact id,
+end⟩⟩
+
+@[simp] lemma contract_next (s : Stream ι α) (q : s.σ) : (Stream.contract s).next q = s.next q := rfl
+
+lemma contract_map {β : Type*} (f : α → β) (s : Stream ι α) :
+  (s.map f).contract = s.contract.map f := rfl
+
+end index_lemmas
+
+section value_lemmas
+variables [add_comm_monoid α]
+
+lemma contract_eval₀ (s : Stream ι α) (q : s.σ) (hq : s.valid q) :
+  (Stream.contract s).eval₀ q hq () = finsupp.sum_range (s.eval₀ q hq) :=
+by { simp only [Stream.eval₀], dsimp, split_ifs with hr; simp, }
+
+lemma contract_eval (s : Stream ι α) [is_bounded s] [add_comm_monoid α] (q : s.σ) :
+  (Stream.contract s).eval q () = finsupp.sum_range (s.eval q) :=
+begin
+  refine @well_founded.induction _ (Stream.contract s).wf_rel (Stream.contract s).wf _ q _,
+  clear q, intros q ih,
+  by_cases hq : s.valid q, swap, { simp [hq], },
+  simp only [s.eval_valid _ hq, (Stream.contract s).eval_valid _ hq, finsupp.coe_add, pi.add_apply,
+    map_add, ih _ ((Stream.contract s).next_wf q hq)], rw [contract_next, contract_eval₀],
+end
+
+lemma contract_mono (s : Stream ι α) : (Stream.contract s).is_monotonic :=
+λ q hq i, by { rw [Stream.index'_val hq, punit_eq_star ((Stream.contract s).index q hq)], exact bot_le, }
+
+instance (s : Stream ι α) [is_lawful s] : is_lawful (Stream.contract s) :=
+{ mono := contract_mono s,
+  skip_spec := λ q hq i j hj, begin
+    cases j,
+    obtain rfl : i = ((), ff) := le_bot_iff.mp hj,
+    simp only [Stream.contract_skip, contract_eval, Stream.eval_skip_eq_of_ff],
+  end }
+
+end value_lemmas
+
+
+
