src/verification/semantics/dense.lean
@@ -1,0 +1,123 @@
+import verification.semantics.skip_stream
+
+/-! 
+# Dense Vectors as Indexed Streams (sanity check)
+
+In this file, we show that `denseVec` (modelling dense vectors as a stream)
+satisfies the stream conditions (it is strictly lawful); therefore our conditions are not vacuous.
+A similar thing can be done for sparse vectors.
+
+This is mostly a lot of tedious casework. TODO: can we automate this to an SMT solver? 
+
+## Definitions:
+We define `Stream.denseVec vals`, which takes a vector `vals` and constructs
+an always-ready stream that outputs the elements of `vals`. The state of `denseVec`
+is considered to be `fin (n + 1)`, the natural numbers `0 ≤ q ≤ n`, where `q : fin (n + 1)` is the terminated state
+
+## Main results:
+  - `Stream.denseVec_eval`: Evaluating from a state `q : fin (n + 1)` results in
+      emitting `vals[q:]` at the appropriate indices.
+        - Corollary (`Stream.denseVec_eval_start`): Starting from `q = 0` produces the whole vector.
+  - `is_strict_lawful (Stream.denseVec vals)`: The stream associated with a dense vector is strictly lawful
+-/
+
+
+
+variables {α : Type*}
+
+def Stream.denseVec {n : ℕ} (vals : fin n → α) : Stream (fin n) α :=
+{ σ := fin (n + 1),
+  valid := λ i, ↑i < n,
+  ready := λ i, ↑i < n,
+  skip := λ i hi j, max i (cond j.2 j.1.succ (fin.cast_le n.le_succ j.1)),
+  index := λ i hi, i.cast_lt hi,
+  value := λ i hi, vals (i.cast_lt hi), }
+
+section
+local attribute [reducible] Stream.denseVec
+
+instance {n} (vals : fin n → α) : is_bounded (Stream.denseVec vals) :=
+⟨⟨(>), finite.preorder.well_founded_gt, λ i hi j, begin
+  simp [Stream.to_order, hi],
+  rcases j with ⟨j, (b|b)⟩,
+  { rw prod.lex.lt_iff'', cases j, cases i, simp, rw [or_iff_not_imp_left, not_lt], tauto, },
+  { rw prod.lex.lt_iff'', cases i, cases j, simp [@lt_iff_not_le _ _ tt, imp_false, ← lt_iff_le_and_ne, nat.lt_succ_iff, nat.succ_le_iff], exact le_or_lt _ _, },
+end⟩⟩
+
+variables [add_zero_class α]
+
+lemma fin.cast_lt_le_iff {m n : ℕ} (a b : fin n) (h₁ : ↑a < m) (h₂ : ↑b < m) :
+  a.cast_lt h₁ ≤ b.cast_lt h₂ ↔ a ≤ b :=
+by { cases a, cases b, simp, }
+
+lemma Stream.denseVec.eq_n_of_invalid {n : ℕ} {vals : fin n → α} {q : fin (n + 1)}
+  (hq : ¬(Stream.denseVec vals).valid q) : ↑q = n := eq_of_le_of_not_lt (nat.lt_succ_iff.mp q.prop) hq
+
+lemma Stream.denseVec_eval {n : ℕ} (vals : fin n → α) (q : fin (n + 1)) :
+  ⇑((Stream.denseVec vals).eval q) = (λ j, if (fin.cast_succ j) < q then 0 else vals j) :=
+begin
+  refine @well_founded.induction _ _ (Stream.denseVec vals).wf _ q _,
+  clear q, intros q ih,
+  by_cases hq : (Stream.denseVec vals).valid q, swap,
+  { replace hq : ↑q = n := Stream.denseVec.eq_n_of_invalid hq,
+    rw [Stream.eval_invalid], swap, { exact hq.not_lt, },
+    ext j,
+    have : (fin.cast_succ j) < q, { rw fin.lt_iff_coe_lt_coe, rw hq, simp, },
+    simp only [this, finsupp.coe_zero, pi.zero_apply, if_true], },
+  { rw [Stream.eval_valid, Stream.eval₀, dif_pos]; try { exact hq },
+    ext j,
+    rw [finsupp.add_apply, ih _ ((Stream.denseVec vals).next_wf q hq)], dsimp only,
+    rcases lt_trichotomy (fin.cast_succ j) q with (h|h|h),
+    { rw [if_pos, add_zero], swap, { simp [Stream.next_val hq], left, assumption, },
+      rw [if_pos], swap, { assumption, },
+      rw finsupp.single_apply_eq_zero, intro h', exfalso, refine h.not_le _,
+      simp [h'], },
+    { have : fin.cast_lt q hq = j, { simp [← h], },
+      rw [if_pos, add_zero], swap, { simp [Stream.next_val hq, (show ↑q < n, from hq)], right, rw this, exact fin.cast_succ_lt_succ _, },
+      rw [if_neg], swap, { exact h.not_lt, },
+      simp [this], },
+    { rw [if_neg], swap, { simp [Stream.next_val hq, (show ↑q < n, from hq), not_or_distrib], revert h, cases j, cases q, simp [nat.succ_le_iff], intro h, exact ⟨h.le, h⟩, },
+      rw [if_neg], swap, { exact h.le.not_lt, },
+      rw [finsupp.single_apply_eq_zero.mpr, zero_add],
+      rintro rfl, exfalso, simpa using h, } },
+end
+
+@[simp] lemma Stream.denseVec_eval_start {n : ℕ} (vals : fin n → α) :
+  ⇑((Stream.denseVec vals).eval 0) = vals :=
+by { rw Stream.denseVec_eval, ext j, simp, }
+
+instance {n} (vals : fin n → α) : is_lawful (Stream.denseVec vals) :=
+{ mono := Stream.is_monotonic_iff.mpr $ λ q hq i hq', by { dsimp, rw fin.cast_lt_le_iff, exact le_max_left _ _, },
+  skip_spec := λ q hq i j hj, begin
+    simp only [Stream.denseVec_eval],
+    by_cases h₁ : fin.cast_succ j < q, { simp [h₁], },
+    rw [if_neg, if_neg], { assumption, },
+    rw [lt_max_iff, not_or_distrib],
+    refine ⟨h₁, _⟩, rw [not_lt],
+    rcases i with ⟨i, (b|b)⟩; simp only [cond],
+    { rw [fin.cast_succ, fin.cast_add, order_embedding.le_iff_le],
+      simpa using hj, },
+    { rw ← fin.cast_succ_lt_iff_succ_le,
+      simpa [prod.lex.le_iff'] using hj, },
+  end }
+
+lemma Stream.denseVec_index'_mono {n} (vals : fin n → α) : strict_mono (Stream.denseVec vals).index' :=
+λ q₁ q₂, begin
+  simp only [Stream.index'], split_ifs with h₁ h₂ h₂,
+  { cases q₁, cases q₂, simp, }, { simp only [with_top.coe_lt_top], exact λ _, trivial, },
+  { simp only [not_top_lt, not_lt, fin.lt_iff_coe_lt_coe, Stream.denseVec.eq_n_of_invalid h₁, imp_false], exact nat.lt_succ_iff.mp q₂.prop, },
+  { simp [Stream.denseVec.eq_n_of_invalid h₁, Stream.denseVec.eq_n_of_invalid h₂, fin.lt_iff_coe_lt_coe], },
+end
+
+instance {n} (vals : fin n → α) : is_strict_lawful (Stream.denseVec vals) :=
+⟨⟨Stream.mono _, λ q hq i hi hr, ne_of_lt begin
+  apply Stream.denseVec_index'_mono,
+  rcases i with ⟨i, b⟩, dsimp only,
+  suffices : q < cond b i.succ (fin.cast_succ i),
+  { rw max_eq_right, { exact this, }, exact this.le, },
+  simp only [Stream.to_order, (show ↑q < n, from hq), to_bool_true_eq_tt] at hi,
+  cases i, cases q, cases b; simpa [nat.lt_succ_iff] using hi,
+end⟩⟩
+
+end
+
