src/verification/semantics/examples.lean
@@ -1,0 +1,42 @@
+import verification.semantics.nested_eval
+
+/-!
+# Examples
+
+This file instantiates the abstract theorems in `LawfulEval`
+in some concrete cases. The examples here correspond to the figures in the paper.
+
+-/
+
+variables {ι₁ ι₂ ι₃ : Type} [linear_order ι₁] [linear_order ι₂]
+  [linear_order ι₃] {R : Type} [semiring R]
+
+open Eval (eval)
+
+example (a b c d : ι₁ ⟶ₛ ι₂ ⟶ₛ ι₃ ⟶ₛ R)  : 
+  eval (a * (b + c) * d) =
+  (eval a) * ((eval b) + (eval c)) * (eval d) :=
+by simp
+
+local notation `∑ᵢ ` s := s.contract
+
+open_locale big_operators
+
+/-- This is the more Lean appropriate way to state the next example -/
+example (a b : ι₁ ⟶ₛ ι₂ ⟶ₛ R) (j : ι₂) :
+  (eval (∑ᵢ (a * b)) : unit →₀ ι₂ →₀ R) () j =
+  (finsupp.sum_range (eval a * eval b) : ι₂ →₀ R) j :=
+by simp
+
+-- Unfortunately, Lean doesn't like the notation `eval s x y` because it doesn't know `eval s x` is going to be a function
+@[reducible] noncomputable def eval₂ {ι₁ ι₂ R : Type*} [linear_order ι₁] [linear_order ι₂] [semiring R]
+  (x : ι₁ ⟶ₛ ι₂ ⟶ₛ R) : ι₁ →₀ ι₂ →₀ R := eval x
+
+/-- This is the same as the previous example, but `finsupp.sum_range` 
+  is changed to a summation notation that might be more understandable
+  because it is closer to "math" notation. -/
+example (a b : ι₁ ⟶ₛ ι₂ ⟶ₛ R) (j : ι₂) :
+  (eval (∑ᵢ (a * b)) : unit →₀ ι₂ →₀ R) () j =
+  ∑ i in (eval₂ a * eval₂ b).support,
+    (eval₂ a i j * eval₂ b i j) :=
+by simp [finsupp.sum_range_eq_sum, finsupp.sum, finsupp.finset_sum_apply]
