src/verification/semantics/nested_eval.lean
@@ -1,0 +1,177 @@
+import verification.semantics.skip_stream
+import verification.semantics.zero
+import verification.semantics.add
+import verification.semantics.mul
+import verification.semantics.contract
+import verification.semantics.replicate
+
+/-!
+# Nested stream evaluation
+
+In this file, we define how nested streams are evaluated.
+To do this, we use Lean's typeclass system to infer an evaluation
+function depending on the shape of the nested stream.
+
+## Main definitions
+  - `BoundedStream`: A stream bundled with an initial state and a proof that the stream is bounded
+  - `LawfulStream`: A stream bundled with a proof that the stream is strictly lawful
+  - `LawfulEval`: An evaluation function that preserves addition, multiplication, and zero
+
+## Main results 
+  - `LawfulEval.ind`: Shows that if `α` lawfully evaluates to `β`,
+      then (lawful) streams of type `ι ⟶ₛ α` lawfully evaluate to
+      finitely supported functions `ι →₀ β`. In the base case, `α = β`,
+      and in the inductive case, `α` is itself another stream type which
+      lawfully evaluates to `β`. This, together with `LawfulStream.eval_contract`
+      and `LawfulStream.eval_replicate`, corresponds to theorem 6.1 in the paper.
+
+-/
+
+noncomputable theory
+open_locale classical
+
+@[ext]
+structure BoundedStream (ι : Type) [linear_order ι] (α : Type*) extends Stream ι α := 
+(init : σ)
+(bdd : is_bounded to_Stream)
+
+infixr ` ⟶b `:50 := BoundedStream
+local notation `↟`s := s.to_Stream
+attribute [instance] BoundedStream.bdd
+
+variables {ι : Type} [linear_order ι] {α β γ : Type*}
+
+@[simps] def BoundedStream.map (f : α → β) (s : BoundedStream ι α) : BoundedStream ι β :=
+BoundedStream.mk (s.map f) s.init (by simp; apply_instance)
+
+@[simp] lemma BoundedStream.map_id (s : BoundedStream ι α) : s.map id = s :=
+by ext : 1; simp
+
+lemma BoundedStream.map_map (g : α → β) (f : β → γ) (s : BoundedStream ι α) :
+  (s.map g).map f = s.map (f ∘ g) :=
+by ext : 1; simp [Stream.map_map]
+
+class Eval (α : Type*) (β : out_param Type*)
+  [add_zero_class β] :=
+(eval : α → β)
+
+open Eval
+
+instance Eval.base {α : Type*} [add_zero_class α] : Eval α α :=
+{ eval := id }
+
+instance Eval.ind (ι : Type) [linear_order ι] (α β : Type*) [add_zero_class β]
+  [Eval α β] : Eval (ι ⟶b α) (ι →₀ β) :=
+{ eval := λ s, (s.map eval).eval s.init  }
+
+structure StrictLawfulStream (ι : Type) [linear_order ι] (α : Type*) {β : Type*} [add_zero_class β]
+  [Eval α β] extends (ι ⟶b α) :=
+(strict_lawful : is_strict_lawful (to_Stream.map eval))
+
+infixr ` ⟶ₛ `:50 := StrictLawfulStream
+
+attribute [instance] StrictLawfulStream.strict_lawful
+
+@[simp] lemma StrictLawfulStream.to_BoundedStream_to_Stream [add_zero_class β] [Eval α β] (s : ι ⟶ₛ α) :
+  (↟(s.to_BoundedStream)) = ↟s := rfl
+
+class LawfulEval (α : Type*) (β : out_param Type*) [non_unital_non_assoc_semiring β]
+  extends Eval α β, has_add α, has_mul α, has_zero α :=
+(eval_zero : eval 0 = 0)
+(eval_add : ∀ x y, eval (x + y) = (eval x) + (eval y))
+(eval_mul : ∀ x y, eval (x * y) = (eval x) * (eval y))
+
+instance LawfulEval.base {α : Type*} [non_unital_non_assoc_semiring α] :
+  LawfulEval α α :=
+{ eval_zero := rfl,
+  eval_add := λ x y, rfl,
+  eval_mul := λ x y, rfl }
+
+@[simps] def BoundedStream.add [has_zero α] [has_add α] (q r : ι ⟶b α) : ι ⟶b α :=
+⟨q.add ↟r, (q.init, r.init), infer_instance⟩
+
+@[simps] def BoundedStream.mul [has_mul α] (q r : ι ⟶b α) : ι ⟶b α :=
+⟨q.mul ↟r, (q.init, r.init), infer_instance⟩
+
+@[simps] def BoundedStream.zero : ι ⟶b α :=
+⟨Stream.zero ι α, (), infer_instance⟩
+
+@[simps] def BoundedStream.contract (s : ι ⟶b α) : unit ⟶b α :=
+⟨(↟s).contract, s.init, infer_instance⟩
+
+@[simps] def BoundedStream.replicate (n : ℕ) (v : α) : (fin n) ⟶b α :=
+⟨Stream.replicate n v, (0 : fin (n + 1)), infer_instance⟩
+
+def Stream.eval' [add_zero_class α] (s : Stream ι α) (q : s.σ) : ι →₀ α :=
+if h : is_bounded s then by resetI; exact s.eval q else classical.arbitrary _
+
+lemma Stream.eval'_eq [add_zero_class α] (s : Stream ι α) [is_bounded s] (q : s.σ) :
+  s.eval' q = s.eval q := dif_pos _
+
+lemma BoundedStream.zero_eval [non_unital_non_assoc_semiring β] [LawfulEval α β] :
+  eval (@BoundedStream.zero ι _ α) = (0 : ι →₀ β) :=
+by { dsimp [eval], rw [← Stream.eval'_eq], convert_to (Stream.zero ι β).eval' () = 0, { congr, simp, }, simp [Stream.eval'_eq], } 
+
+lemma Stream.add_map_eval [non_unital_non_assoc_semiring β] [LawfulEval α β] :
+  ∀ (q r : Stream ι α), (q.add r).map eval = ((q.map eval).add (r.map eval)) :=
+Stream.add_map eval LawfulEval.eval_add LawfulEval.eval_zero
+
+lemma Stream.mul_map_eval [non_unital_non_assoc_semiring β] [LawfulEval α β] :
+  ∀ (q r : Stream ι α), (q.mul r).map eval = ((q.map eval).mul (r.map eval)) :=
+Stream.mul_map eval LawfulEval.eval_mul
+
+lemma BoundedStream.add_map_eval [non_unital_non_assoc_semiring β] [LawfulEval α β] (q r : ι ⟶b α) :
+  (q.add r).map eval = ((q.map eval).add (r.map eval)) :=
+by { ext : 1, { exact Stream.add_map_eval (↟q) (↟r), }, refl, }
+
+lemma BoundedStream.mul_map_eval [non_unital_non_assoc_semiring β] [LawfulEval α β] (q r : ι ⟶b α) :
+  (q.mul r).map eval = ((q.map eval).mul (r.map eval)) :=
+by { ext : 1, { exact Stream.mul_map_eval _ _, }, refl, }
+
+lemma BoundedStream.eval_add [non_unital_non_assoc_semiring β] [LawfulEval α β]
+  (q r : ι ⟶b α) [is_lawful ((↟q).map eval)] [is_lawful ((↟r).map eval)] : eval (q.add r) = (eval q) + (eval r) :=
+begin
+  dsimp only [eval], conv_lhs { rw ← Stream.eval'_eq, },
+  convert_to ((q.map eval).add (r.map eval)).eval' (q.add r).init = _,
+  { congr, exact BoundedStream.add_map_eval q r, },
+  rw Stream.eval'_eq, dsimp, rw add_spec,
+end
+
+lemma BoundedStream.eval_contract [non_unital_non_assoc_semiring β] [LawfulEval α β]
+  (q : ι ⟶b α) [is_lawful ((↟q).map eval)] : (eval q.contract : unit →₀ β) () = finsupp.sum_range (eval q) :=
+by { dsimp [eval, ← contract_map], exact contract_eval _ _, }
+
+lemma BoundedStream.eval_mul [non_unital_non_assoc_semiring β] [LawfulEval α β]
+  (q r : ι ⟶b α) [is_strict_lawful ((↟q).map eval)] [is_strict_lawful ((↟r).map eval)] :
+  eval (q.mul r) = (eval q) * (eval r) :=
+begin
+  dsimp only [eval], conv_lhs { rw ← Stream.eval'_eq, },
+  convert_to ((q.map eval).mul (r.map eval)).eval' (q.mul r).init = _,
+  { congr, exact BoundedStream.mul_map_eval q r, },
+  rw Stream.eval'_eq, dsimp, rw mul_spec,
+end
+
+@[simps] def LawfulStream.replicate [non_unital_non_assoc_semiring β] [LawfulEval α β]
+  (n : ℕ) (v : α) : (fin n) ⟶ₛ α :=
+⟨BoundedStream.replicate n v, (by { dsimp, apply_instance, })⟩
+
+instance LawfulEval.ind [non_unital_non_assoc_semiring β]
+  [LawfulEval α β] : LawfulEval (ι ⟶ₛ α) (ι →₀ β) :=
+{ eval := λ s, eval s.to_BoundedStream,
+  add := λ x y, ⟨x.add y.to_BoundedStream, by { dsimp, rw Stream.add_map_eval, apply_instance, }⟩,
+  mul := λ x y, ⟨x.mul y.to_BoundedStream, by { dsimp, rw Stream.mul_map_eval, apply_instance, }⟩,
+  zero := ⟨BoundedStream.zero, by { simp, apply_instance, }⟩,
+  eval_zero := BoundedStream.zero_eval,
+  eval_add := λ x y, BoundedStream.eval_add _ _,
+  eval_mul := λ x y, BoundedStream.eval_mul _ _ }
+
+attribute [simp] LawfulEval.eval_add LawfulEval.eval_zero
+  LawfulEval.eval_mul
+
+@[simp] lemma LawfulStream.eval_contract [non_unital_non_assoc_semiring β]
+  [LawfulEval α β] (q : ι ⟶ₛ α) : (eval q.contract : unit →₀ β) () = finsupp.sum_range (eval q) :=
+BoundedStream.eval_contract _
+
+@[simp] lemma LawfulStream.eval_replicate [non_unital_non_assoc_semiring β]
+  [LawfulEval α β] (n : ℕ) (v : α) (j : fin n) : (eval (LawfulStream.replicate n v) : fin n →₀ β) j = eval v :=
+by { dsimp [eval], simp, }
