src/verification/semantics/replicate.lean
@@ -1,0 +1,30 @@
+import verification.semantics.dense
+
+/-!
+# Stream replicate
+
+This file defines replicate, which is a specialization of the dense vector 
+stream to a constant function.
+
+**Note: the current version of the paper uses the terminology *expand*, which was from a previous version of the paper.
+The terms *replicate* and *expand* should be considered to be synonymous**.
+
+-/
+
+variables {α β : Type*}
+
+@[derive is_bounded]
+def Stream.replicate (n : ℕ) (v : α) : Stream (fin n) α :=
+Stream.denseVec (λ _, v)
+
+@[simp] lemma Stream.replicate_map (f : α → β) (n : ℕ) (v : α) :
+  (Stream.replicate n v).map f = Stream.replicate n (f v) := rfl
+
+variables [add_zero_class α]
+
+instance (n : ℕ) (v : α) : is_strict_lawful (Stream.replicate n v) :=
+by { dunfold Stream.replicate, apply_instance, }
+
+@[simp] lemma Stream.replicate_eval (n : ℕ) (v : α) (j : fin n) :
+  (Stream.replicate n v).eval (0 : fin (n + 1)) j = v :=
+by { dunfold Stream.replicate, simp, }
